utils/theories/SemiLattice.v
@@ -1,0 +1,120 @@
+(* Distributed under the terms of the MIT license. *)
+From Stdlib Require Import ssreflect ssrbool ZArith.
+From Stdlib Require Import Program RelationClasses Morphisms.
+From Stdlib Require Import Orders OrderedTypeAlt OrderedTypeEx MSetList MSetInterface MSetAVL MSetFacts FMapInterface MSetProperties MSetDecide.
+From MetaRocq.Utils Require Import utils NonEmptyLevelExprSet.
+
+Module Semilattice.
+  Declare Scope sl_scope.
+  Open Scope sl_scope.
+
+  Reserved Notation "x ≡ y" (at level 90).
+  Class Semilattice (carrier : Type) :=
+    { eq : carrier -> carrier -> Prop where "x ≡ y" := (eq x y) : sl_scope;
+      eq_equiv :: Equivalence eq;
+      add : Z -> carrier -> carrier;
+      join : carrier -> carrier -> carrier;
+      add_distr n m x : add n (add m x) ≡ add (n + m) x;
+      add_neutral x : add 0 x ≡ x;
+      join_assoc x y z : join (join x y) z ≡ join x (join y z);
+      join_comm x y : join x y ≡ join y x;
+      join_congr x x' y : x ≡ x' -> join x y ≡ join x' y;
+      join_idem x : join x x ≡ x;
+      join_sub x : join x (add 1 x) ≡ add 1 x;
+      succ_inj : forall n x y, add n x ≡ add n y -> x ≡ y;
+      succ_join : forall n x y, add n (join x y) ≡ join (add n x) (add n y);
+    }.
+
+  Notation "x ≡ y" := (eq x y) (at level 90) : sl_scope.
+
+  Definition le {A} {SL : Semilattice A} (x y : A) := join x y ≡ y.
+
+  Infix "≤" := le (at level 50) : sl_scope.
+  Infix "∨" := join (at level 30) : sl_scope.
+
+  Local Open Scope nat_scope.
+  Section Derived.
+    Context {A : Type} {SL : Semilattice A}.
+
+    Lemma join_congr_r x y y' : y ≡ y' -> join x y ≡ join x y'.
+    Proof.
+      intros he; etransitivity. apply join_comm.
+      etransitivity. 2:apply join_comm. now apply join_congr.
+    Qed.
+
+    #[export] Instance proper_join : Proper (eq ==> eq ==> eq) join.
+    Proof. intros x y ? x0 y0 ?. transitivity (join y x0).
+      now apply join_congr. now apply join_congr_r.
+    Qed.
+
+    Lemma le_refl x : x ≤ x.
+    Proof. apply join_idem. Qed.
+    Lemma le_trans x y z : x ≤ y -> y ≤ z -> x ≤ z.
+    Proof.
+      unfold le; intros le le'. now rewrite -le' -join_assoc le.
+    Qed.
+    #[export] Instance le_preorder : PreOrder le.
+    Proof.
+      split.
+      - intros ?; apply le_refl.
+      - intros ? ? ?. apply le_trans.
+    Qed.
+
+    Lemma eq_antisym {x y} : x ≡ y <-> x ≤ y /\ y ≤ x.
+    Proof.
+      split.
+      - intros he. split.
+        red. rewrite -he. apply join_idem.
+        red. rewrite -he. apply join_idem.
+      - intros [le le'].
+        red in le, le'. rewrite -le. rewrite -{1}le'.
+        apply join_comm.
+    Qed.
+
+    #[export] Instance proper_le : Proper (eq ==> eq ==> iff) le.
+    Proof. intros x y ? x0 y0 ?.
+      apply eq_antisym in H0 as [].
+      apply eq_antisym in H as [].
+      split.
+      - intros leq. transitivity x => //. transitivity x0 => //.
+      - intros le. transitivity y => //. transitivity y0 => //.
+    Qed.
+
+    #[export] Instance po : PartialOrder eq le.
+    Proof.
+      split.
+      - intros eq; split. now rewrite eq. red.
+        now rewrite eq.
+      - intros []. red in H0. apply eq_antisym. split => //.
+    Qed.
+
+    Lemma join_le_left {s t} : s ≤ s ∨ t.
+    Proof.
+      red. now rewrite -join_assoc join_idem.
+    Qed.
+
+    Lemma join_le_right {s t} : t ≤ s ∨ t.
+    Proof.
+      rewrite join_comm; apply join_le_left.
+    Qed.
+
+    Lemma join_le_left_eq {s t u} :
+      s ∨ t ≤ u <-> s ≤ u /\ t ≤ u.
+    Proof.
+      split.
+      - intros le; split; transitivity (s ∨ t) => //. apply join_le_left.
+        apply join_le_right.
+      - intros [le le']. red in le, le'. red.
+        now rewrite join_assoc le' le.
+    Qed.
+
+    Lemma join_le_right_impl {s t u} :
+      s ≤ t \/ s ≤ u -> s ≤ t ∨ u.
+    Proof.
+      intros [le|le]; red in le; red.
+      now rewrite -join_assoc le.
+      now rewrite (join_comm t) -join_assoc le.
+    Qed.
+
+  End Derived.
+End Semilattice.
